lava/out/Benchmark/RBinsToBins.v
@@ -95,13 +95,13 @@ Defined.
 #[global] Hint Unfold RZ: ref_constr_db.
 
 Inductive Bin_u: Type :=
-  | B0_u: Bin_u → Bin_u | B1_u: Bin_u → Bin_u | Z_u: Bin_u.
+  | B0_u: Bin_u → Bin_u | B1_u: Bin_u → Bin_u | RBinsToBins__Z_u: Bin_u.
 
 Fixpoint Bin_eq (x y : Bin_u): bool :=
   match (x, y) with
   | (B0_u n, B0_u n') => true && Bin_eq n n'
   | (B1_u n, B1_u n') => true && Bin_eq n n'
-  | (Z_u, Z_u) => true
+  | (RBinsToBins__Z_u, RBinsToBins__Z_u) => true
   | (_, _) => false
   end.
 
@@ -125,7 +125,11 @@ Qed.
     eqb_eq' := Bin_eqb_eq }.
 
 Fixpoint Bin_wf (x : Bin_u): Prop :=
-  match x with | B0_u n => Bin_wf n ∧ True | B1_u n => Bin_wf n ∧ True | Z_u => True end.
+  match x with
+  | B0_u n => Bin_wf n ∧ True
+  | B1_u n => Bin_wf n ∧ True
+  | RBinsToBins__Z_u => True
+  end.
 
 Theorem Bin_wf_ref [p : Bin_u → Prop] (tm : {v: Bin_u | Bin_wf v ∧ p v}): Bin_wf ⌊ tm -⌋.
 Proof.
@@ -150,13 +154,13 @@ Defined.
 Definition B1 (n : Bin): Bin :=
   exist _ (B1_u ⌊ n -⌋) (B1_lem n).
 
-Definition Z_lem : Bin_wf Z_u ∧ True.
+Definition RBinsToBins__Z_lem : Bin_wf RBinsToBins__Z_u ∧ True.
 Proof.
   repeat first [split | solver].
 Defined.
 
-Definition Z : Bin :=
-  exist _ Z_u Z_lem.
+Definition RBinsToBins__Z : Bin :=
+  exist _ RBinsToBins__Z_u RBinsToBins__Z_lem.
 
 Definition wf_B0_n [n : Bin_u] (p : Bin_wf (B0_u n)): Bin_wf n.
 Proof.
@@ -182,7 +186,7 @@ Defined.
 
 #[global] Hint Unfold B1: ref_constr_db.
 
-#[global] Hint Unfold Z: ref_constr_db.
+#[global] Hint Unfold RBinsToBins__Z: ref_constr_db.
 
 Definition rbinToBin_spec (ds_d4Ff : RBin): Type :=
   Bin.
@@ -195,5 +199,5 @@ Proof.
   induction ds_d4Ff as [n IH_n| n IH_n|].
   - refine (B0 (IH_n ltac:(try clear IH_n; solver))).
   - refine (B1 (IH_n ltac:(try clear IH_n; solver))).
-  - refine Z.
+  - refine RBinsToBins__Z.
 Defined.
